clean up repo + restate message definition

src/program_proof/session/definitions.v
@@ -1,6 +1,4 @@
-From Goose.github_com.session Require Export server.
-From Perennial.program_proof Require Export std_proof.
-From Perennial.program_proof Require Export grove_prelude.
+From Perennial.program_proof.session Require Export session_prelude.
 
 Module Operation.
   
@@ -39,6 +37,7 @@ Module Message.
 	          S2C_Client_OperationType: u64;    
 	          S2C_Client_Data:          u64;
 	          S2C_Client_VersionVector: list u64;
+                  S2C_Server_Id:            u64;
 	          S2C_Client_Number:        u64;
                 }.
 
@@ -68,9 +67,7 @@ Section heap.
 
   Theorem operation_val_t op : val_ty (operation_val op) (struct.t Operation).
   Proof.
-    repeat constructor.
-    destruct op. simpl.
-    val_ty.
+    repeat constructor; auto.
   Qed.
 
   Hint Resolve operation_val_t : core.
@@ -91,7 +88,7 @@ Section heap.
     destruct v as [[a []] d]; done. 
   Defined. 
 
-  #[global] Instance into_val_for_type : IntoValForType (Slice.t*u64) (struct.t Operation).
+  #[global] Instance operation_into_val_for_type : IntoValForType (Slice.t*u64) (struct.t Operation).
   Proof. constructor; auto. Qed.
 
   Definition is_operation (opv: Slice.t*u64) (op: Operation.t) (opv_len: nat): iProp Σ :=
@@ -109,5 +106,55 @@ Section heap.
 
   Definition operation_to_val (o: Operation.t) (s: Slice.t) :=
     (s, (#o.(Operation.Data), #()))%V.
+
+  Definition message_val (msg:u64*u64*u64*u64*u64*Slice.t*u64*u64*Slice.t*u64*u64*u64*u64*u64*u64*Slice.t*u64*u64) : val :=
+    (#msg.1.1.1.1.1.1.1.1.1.1.1.1.1.1.1.1.1,
+       (#msg.1.1.1.1.1.1.1.1.1.1.1.1.1.1.1.1.2,
+          (#msg.1.1.1.1.1.1.1.1.1.1.1.1.1.1.1.2,
+             (#msg.1.1.1.1.1.1.1.1.1.1.1.1.1.1.2,
+                (#msg.1.1.1.1.1.1.1.1.1.1.1.1.1.2,
+                   (slice_val msg.1.1.1.1.1.1.1.1.1.1.1.1.2,
+                      (#msg.1.1.1.1.1.1.1.1.1.1.1.2,
+                         (#msg.1.1.1.1.1.1.1.1.1.1.2,
+                            (slice_val msg.1.1.1.1.1.1.1.1.1.2,
+                               (#msg.1.1.1.1.1.1.1.1.2,
+                                  (#msg.1.1.1.1.1.1.1.2,
+                                     (#msg.1.1.1.1.1.1.2,
+                                        (#msg.1.1.1.1.1.2,
+                                           (#msg.1.1.1.1.2,
+                                              (#msg.1.1.1.2,
+                                                 (slice_val msg.1.1.2,
+                                                    (#msg.1.2,
+                                                       (#msg.2, #()))))))))))))))))))%V.
+
+  Theorem message_val_t msg : val_ty (message_val msg) (struct.t server.Message).
+  Proof.
+    repeat constructor; auto.
+  Qed.
+
+  Hint Resolve message_val_t : core.
+  
+  Definition is_message (msgv: u64*u64*u64*u64*u64*Slice.t*u64*u64*Slice.t*u64*u64*u64*u64*u64*u64*Slice.t*u64*u64)
+    (msg: Message.t) (msgv_len: nat): iProp Σ :=
+    ⌜msgv.1.1.1.1.1.1.1.1.1.1.1.1.1.1.1.1.1 = msg.(Message.MessageType)⌝ ∗
+    ⌜msgv.1.1.1.1.1.1.1.1.1.1.1.1.1.1.1.1.2 = msg.(Message.C2S_Client_Id)⌝ ∗
+    ⌜msgv.1.1.1.1.1.1.1.1.1.1.1.1.1.1.1.2 = msg.(Message.C2S_Server_Id)⌝ ∗
+    ⌜msgv.1.1.1.1.1.1.1.1.1.1.1.1.1.1.2 = msg.(Message.C2S_Client_OperationType)⌝ ∗
+    ⌜msgv.1.1.1.1.1.1.1.1.1.1.1.1.1.2 = msg.(Message.C2S_Client_Data)⌝ ∗
+    ⌜msgv_len = length msg.(Message.C2S_Client_VersionVector)⌝ ∗
+    own_slice_small msgv.1.1.1.1.1.1.1.1.1.1.1.1.2 uint64T DfracDiscarded msg.(Message.C2S_Client_VersionVector) ∗
+    ⌜msgv.1.1.1.1.1.1.1.1.1.1.1.2 = msg.(Message.S2S_Gossip_Sending_ServerId)⌝ ∗
+    ⌜msgv.1.1.1.1.1.1.1.1.1.1.2 = msg.(Message.S2S_Gossip_Receiving_ServerId)⌝ ∗
+    operation_slice msgv.1.1.1.1.1.1.1.1.1.2 msg.(Message.S2S_Gossip_Operations) msgv_len ∗
+    ⌜msgv.1.1.1.1.1.1.1.1.2 = msg.(Message.S2S_Gossip_Index)⌝ ∗
+    ⌜msgv.1.1.1.1.1.1.1.2 = msg.(Message.S2S_Acknowledge_Gossip_Sending_ServerId)⌝ ∗
+    ⌜msgv.1.1.1.1.1.1.2 = msg.(Message.S2S_Acknowledge_Gossip_Receiving_ServerId)⌝ ∗
+    ⌜msgv.1.1.1.1.1.2 = msg.(Message.S2S_Acknowledge_Gossip_Index)⌝ ∗
+    ⌜msgv.1.1.1.1.2 = msg.(Message.S2C_Client_OperationType)⌝ ∗
+    ⌜msgv.1.1.1.2 = msg.(Message.S2C_Client_Data)⌝ ∗
+    ⌜msgv_len = length msg.(Message.S2C_Client_VersionVector)⌝ ∗
+    own_slice_small msgv.1.1.2 uint64T DfracDiscarded msg.(Message.S2C_Client_VersionVector) ∗
+    ⌜msgv.1.2 = msg.(Message.S2C_Server_Id)⌝ ∗
+    ⌜msgv.2 = msg.(Message.S2C_Client_Number)⌝.
 
 End heap.
