src/program_proof/session/coq_session.v
@@ -132,13 +132,14 @@ Definition coq_getGossipOperations (s: Server.t) (serverId: u64) : (list Operati
 Definition coq_processClientRequest (s: Server.t) (r: Message.t) :
   (bool * Server.t * Message.t) :=
   if (negb (coq_compareVersionVector s.(Server.VectorClock) r.(Message.C2S_Client_VersionVector))) then
-    (false, s, (Message.mk 0 0 0 0 0 [] 0 0 [] 0 0 0 0 0 0 [] 0))
+    (false, s, (Message.mk 0 0 0 0 0 [] 0 0 [] 0 0 0 0 0 0 [] 0 0))
   else
     if (uint.nat r.(Message.C2S_Client_OperationType) =? 0) then
       let S2C_Client_Data : u64 := coq_getDataFromOperationLog s.(Server.OperationsPerformed) in
       let S2C_Client_VersionVector : (list u64) := s.(Server.VectorClock) in
       let S2C_Client_Number : u64 := r.(Message.C2S_Client_Id) in
-      (true, s, (Message.mk 4 0 0 0 0 [] 0 0 [] 0 0 0 0 0 S2C_Client_Data S2C_Client_VersionVector S2C_Client_Number))
+      let S2C_Server_Id : u64 := s.(Server.Id) in
+      (true, s, (Message.mk 4 0 0 0 0 [] 0 0 [] 0 0 0 0 0 S2C_Client_Data S2C_Client_VersionVector S2C_Server_Id S2C_Client_Number))
     else
       let v : nat := uint.nat (list_lookup_total (uint.nat s.(Server.Id)) s.(Server.VectorClock)) in
       let VectorClock : list u64 := <[(uint.nat s.(Server.Id))%nat := (W64 (v + 1))]>s.(Server.VectorClock) in
@@ -148,7 +149,8 @@ Definition coq_processClientRequest (s: Server.t) (r: Message.t) :
       let S2C_Client_Data := 0 in
       let S2C_Client_VersionVector := VectorClock in
       let S2C_Client_Number := r.(Message.C2S_Client_Id) in
-      (true, Server.mk s.(Server.Id) s.(Server.NumberOfServers) s.(Server.UnsatisfiedRequests) VectorClock OperationsPerformed MyOperations s.(Server.PendingOperations) s.(Server.GossipAcknowledgements), (Message.mk 4 0 0 0 0 [] 0 0 [] 0 0 0 0 1 S2C_Client_Data S2C_Client_VersionVector S2C_Client_Number)).
+      let S2C_Server_Id : u64 := s.(Server.Id) in
+      (true, Server.mk s.(Server.Id) s.(Server.NumberOfServers) s.(Server.UnsatisfiedRequests) VectorClock OperationsPerformed MyOperations s.(Server.PendingOperations) s.(Server.GossipAcknowledgements), (Message.mk 4 0 0 0 0 [] 0 0 [] 0 0 0 0 1 S2C_Client_Data S2C_Client_VersionVector S2C_Server_Id S2C_Client_Number)).
 
 Definition coq_processRequest (s: Server.t) (r: Message.t) : (Server.t * list Message.t) :=
   match (uint.nat r.(Message.MessageType))%nat with
@@ -162,7 +164,7 @@ Definition coq_processRequest (s: Server.t) (r: Message.t) : (Server.t * list Me
         (server, [])
   | 1%nat =>
       let s := coq_receiveGossip s r in
-      let outGoingRequests := [Message.mk 0 0 0 0 0 [] 0 0 [] 0 (s.(Server.Id)) (r.(Message.S2S_Gossip_Sending_ServerId)) (r.(Message.S2S_Gossip_Index)) 0 0 [] 0] in
+      let outGoingRequests := [Message.mk 0 0 0 0 0 [] 0 0 [] 0 (s.(Server.Id)) (r.(Message.S2S_Gossip_Sending_ServerId)) (r.(Message.S2S_Gossip_Index)) 0 0 [] 0 0] in
       let '(_, deletedIndex, outGoingRequests) := fold_left (fun (acc: nat * list nat * list Message.t) element =>
                                            let '(index, deletedIndex, acc) := acc in
                                            let '(succeeded, server, reply) := coq_processClientRequest s r in
@@ -190,7 +192,7 @@ Definition coq_processRequest (s: Server.t) (r: Message.t) : (Server.t * list Me
                                               let S2S_Gossip_Receiving_ServerId := index in
                                               let S2S_Gossip_Operations := coq_getGossipOperations s index in
                                               let S2S_Gossip_Index := length (s.(Server.MyOperations)) in
-                                              let message := Message.mk 1 0 0 0 0 [] S2S_Gossip_Sending_ServerId S2S_Gossip_Receiving_ServerId S2S_Gossip_Operations S2S_Gossip_Index 0 0 0 0 0 [] 0 in acc ++ [message]
+                                              let message := Message.mk 1 0 0 0 0 [] S2S_Gossip_Sending_ServerId S2S_Gossip_Receiving_ServerId S2S_Gossip_Operations S2S_Gossip_Index 0 0 0 0 0 [] 0 0 in acc ++ [message]
                                             else
                                               acc) (seq 0 (uint.nat s.(Server.NumberOfServers)))  [] in
       (s, outGoingRequests)
